Slightly revise delimiter format.

src/Narcissus/Formats/Delimiter.v
@@ -18,8 +18,8 @@ Section Delimiter.
   Context {monoid : Monoid T}.
   Context {monoidUnit : QueueMonoidOpt monoid bool}.
 
-  (* [open] should be a format in the future to support XML tag with
-  attributes. *)
+  (* [open] and [close] will probably be formats in the future to support XML
+  tag with attributes and whitespaces. *)
   Variable open : string.
   Variable close : string.
 
@@ -28,38 +28,38 @@ Section Delimiter.
   Variable A_cache_OK : cache_inv_Property A_cache_inv
                                            (fun P => forall b cd, P cd -> P (addD cd b)).
 
-  Definition format_with_term_string : FormatM A T :=
+  Definition format_with_term (close : string) : FormatM A T :=
     format_A ++ format_string ◦ (constant close).
 
   Definition format_delimiter : FormatM A T :=
-    format_string ◦ (constant open) ++ format_with_term_string.
+    format_string ◦ (constant open) ++ format_with_term close.
 
   (* TODO: it is faster to take the size of [open]. *)
   Definition decode_delimiter
-             (decode_with_term_string :
+             (decode_with_term :
                string -> T -> CacheDecode -> option (A * T * CacheDecode))
              (b : T) (cd : CacheDecode)
     : option (A * T * CacheDecode) :=
     `(s, b1, e1) <- decode_string (length open) b cd;
     if String.eqb open s
-    then decode_with_term_string close b1 e1
+    then decode_with_term close b1 e1
     else None.
 
   Theorem delimiter_decode_correct
-          (decode_A_with_term_string
+          (decode_A_with_term
             : string -> T -> CacheDecode -> option (A * T * CacheDecode))
           (A_predicate : string -> A -> Prop)
     : CorrectDecoder monoid (A_predicate close) (A_predicate close)
-                     eq format_with_term_string
-                     (decode_A_with_term_string close)
+                     eq (format_with_term close)
+                     (decode_A_with_term close)
                      A_cache_inv
-                     format_with_term_string ->
+                     (format_with_term close) ->
       CorrectDecoder monoid
                      (A_predicate close)
                      (A_predicate close)
                      eq
                      format_delimiter
-                     (decode_delimiter decode_A_with_term_string)
+                     (decode_delimiter decode_A_with_term)
                      A_cache_inv
                      format_delimiter.
   Proof.
@@ -94,7 +94,7 @@ Section Delimiter.
       eapply DecodeBindOpt2_under_bind.
       intros.
       destruct String.eqb; subst; simpl;
-        destruct decode_A_with_term_string; destruct_conjs; reflexivity.
+        destruct decode_A_with_term; destruct_conjs; reflexivity.
   Qed.
 
 
@@ -107,7 +107,7 @@ Section Delimiter.
                                         format_A.
 
   (* TODO: again, we should take the size of [close]. *)
-  Definition decode_with_term_string_simple (close : string)
+  Definition decode_with_term_simple (close : string)
              (b : T) (cd : CacheDecode)
     : option (A * T * CacheDecode) :=
     `(a, b1, e1) <- decode_A b cd;
@@ -116,15 +116,15 @@ Section Delimiter.
     then Some (a, b2, e2)
     else None.
 
-  Theorem decode_with_term_string_simple_correct
+  Theorem decode_with_term_simple_correct
     : CorrectDecoder monoid A_predicate A_predicate
-                     eq format_with_term_string
-                     (decode_with_term_string_simple close)
+                     eq (format_with_term close)
+                     (decode_with_term_simple close)
                      A_cache_inv
-                     format_with_term_string.
+                     (format_with_term close).
   Proof.
     eapply format_decode_correct_EquivDecoder_Proper; cycle 1.
-    - unfold format_with_term_string.
+    - unfold format_with_term.
       eapply format_decode_correct_refineEquiv; unfold flip.
 
       apply EquivFormat_UnderSequence'.
@@ -148,14 +148,14 @@ Section Delimiter.
 
     - intros t cd.
       unfold sequence_Decode.
-      unfold decode_with_term_string_simple.
+      unfold decode_with_term_simple.
       eapply DecodeBindOpt2_under_bind. intros.
       eapply DecodeBindOpt2_under_bind. intros.
       destruct String.eqb; subst; simpl; reflexivity.
   Qed.
 
   Definition decode_delimiter_simple :=
-    decode_delimiter decode_with_term_string_simple.
+    decode_delimiter decode_with_term_simple.
 
   Corollary delimiter_decode_simple_correct
     : CorrectDecoder monoid
@@ -167,7 +167,7 @@ Section Delimiter.
                      format_delimiter.
   Proof.
     eapply delimiter_decode_correct with (A_predicate := (fun _ => A_predicate)).
-    eapply decode_with_term_string_simple_correct.
+    eapply decode_with_term_simple_correct.
   Qed.
 
 End Delimiter.
